---
title: "Prism Pair "
author:
  - Ryuichi Arafune
keywords: [GVD, GDD, Prism Pair]
format:
  html:
    toc: true
    math: mathjax
    mathjax:
      tex:
        tags: all
    html:
      eqn-number: all
  pdf:
    pdf-engine: lualatex
    toc: true
    classoption: a4paper
    geometry:
      - margin=25mm
abstract: |
  This note describes how to calculate the dispersion characteristics of a prism pair.
execute:
  enabled: true
jupyter: python3
---

# Geometry of Prism Pair

![Prism Pair Geometry](PrismPair_geometry.svg){#fig-prism-pair-geometry}

@fig-prism-pair-geometry shows the geometry of a prism pair. 
Set the apex of the first prism ($O_1$) as the origin of the coordinate system.
And the base is parallel to the $x$-axis of the coordinate system.
The second prism apex ($O_2$) is located at $(W, -H)$ ($H>0,\, W>0$).
And for convenience, the unit vectors $\boldsymbol{u}_1$, $\boldsymbol{u}_2$ and $\boldsymbol{u}_3$ a are defined as shown in @fig-prism-pair-geometry.
The apex angle of the prism is $\alpha$, and the refractive index is $n$.
Both base of the prisms are parallel to each other.
The incident angle and the refraction angle at the first surface of the prism (at Point A) are $\theta_0$ and $\theta_1$,
respectively.
The refraction angles at the second surface (at Point B) are $\theta_2$ and $\theta_3$.
On the second prism, the refraction angles at Point C are $\theta_4$ and $\theta_5$, and 
at Point D are $\theta_6$ and $\theta_7$.
The angles are related by Snell's law.

The GDD is described as follows:
$$
GDD = \frac{\lambda^3}{2 \pi c^2} \frac{d^2 }{d \lambda^2} \left[n(\lambda) (P_{AB}+ P_{CD})+ P_{BC}\right] \times 2
$${#eq-gdd}
where, $P_{AB}$ is the path length in the first prism, $P_{CD}$ is the path length in the second prism, and $P_{BC}$ is the path length in the air between the two prisms.
The factor 2 accounts for the symmetric double-pass geometry.
The ray is incident on the first prism at point A, and exits from the second prism at point D.
The path $P_{O_1A}$ and $P_{O_2C}$ are the input parameters.

Further, the incident angle $\theta_0$ is also the input parameter.

And the distance between the two prisms $W$ and $H$ are also the input parameters.
(Or other quantity that describes the distance between the two prisms may be appropriate.)

$$
\begin{aligned}
P_{O_1 O_2} &= \sqrt{W^2 + H^2}\\
\end{aligned}
$$



$$
\begin{aligned}
\theta_1 + \theta_2 &= \alpha \\
\theta_3 &= \theta_4 \\
\theta_2 &= \theta_5 \\
\theta_1 &= \theta_6 \\
\theta_0 &= \theta_7
\end{aligned}
$$

# Physical distance between A and B (In the prism)

As $P_{AB} \cos\theta_2 = P_{O_1A} \sin \alpha$,
$$
P_{AB} = P_{O_1 A} \frac{\sin \alpha}{\cos\theta_2}
$$ {#eq-PAB}



$P_{O_1 B}$ is the length between the apex and the exit point of the ray in the first prism. 
As, $P_{O_1 B} = P_{O_1 A} \cos \alpha + P_{AB} \sin \theta_2$, thus

$P_{O_1B} = P_{O_1A}\frac{\cos \theta_1}{\cos \theta_2}$ 


# Physical distance between C and D (In the prism)

Likewise, $P_{CD}$ can be calculated as follows:

$$
P_{CD} = P_{O_2 C} \frac{\sin \alpha}{\cos \theta_6} = P_{O_2 C} \frac{\sin \alpha}{\cos \theta_1}
$$ {#eq-PCD}

$P_{O_2C}$ does not depend on the wavelength, $\theta_1$ depends on lambda.

# Physical distance between B and C (In air)

The projection of $BC$ to $\boldsymbol{u}_2$ is same as the projection of $O_1 O_2$ to $\boldsymbol{u}_2$.
The length is $s$ (The gap distance between the prism pair along $\boldsymbol{u}_2$).

$\boldsymbol{u}_2  = (\cos \alpha/2, \sin \alpha /2)$
and
$O_1 O_2 = (W, -H)$, 

Thus, 
$$
\begin{aligned}
P_{BC} \cos \theta_3 = \boldsymbol{u}_2 \cdot O_1 O_2 = W \cos (\alpha/2) - H \sin (\alpha/2)
\end{aligned}
$$

$$
P_{BC} = \frac{W \cos (\alpha/2) - H \sin (\alpha/2)}{\cos \theta_3}
$$ {#eq-PBC}


# Dependency of Prism Separation Parameters

As W and H which determines the distance between the two prisms, $P_{O_1 A}$ and $P_{O_2 C}$ which are the length between the incident point of each prism, are input parameters,
and they can be measured directly.  $\alpha$ is given. $n(\lambda)$ is calculable. Thus, to calculate @eq-gdd, it seems to be completely straight forward.
However, there is a problem here.

$W$, $H$, $P_{O_1 A}$ and $P_{O_2 C}$  are not independent.

One way to overcome this difficulty is taking $O_1 O_2$ instead of $W$ and $H$. However, square root appears in the expression, and it is not convenient.
Thus, the other way is taken: the projection of $O_1 O_2$ along $\boldsymbol{u}_3 = (\sin \alpha/2, -\cos \alpha/2)$:
$$
t \equiv O_1 O_2 \cdot \boldsymbol{u}_3 = W \sin (\alpha/2) + H \cos (\alpha/2).
$$
While the length $t$ is not so easy to measure directly,
it is free from the problem mentioned above, and its quantity is similar size of the apex distance of the prism.

Thus, the other way is taken: the projection $O_1 O_2$ along $\boldsymbol{u}_1 = (\cos \alpha/2, -\sin \alpha/2)$:

\begin{equation}
t_2 \equiv O_1 O_2 \cdot \boldsymbol{u}_1 = W \cos (\alpha/2) + H \sin (\alpha/2).
\end{equation}
While the length $t_2$ is not so easy to measure directly,
it is free from the problem mentioned above, and its quantity is similar size of the apex distance of the prism.

Thus, the problem is how to determine $W$ and $H$ using $t_2$, and $P_{O_1 A}$ and $P_{O_2 C}$ as input parameters.
Once, the $W$ and $H$ are determined, as $\theta_3$ can be determined, and then $P_{BC}$ can be calculated.
Note that material dispersion does not need to be taken into account to determine $W$ and $H$ from $t_2$ and $P_{O_1}$ and $P_{O_2}$.

## Relation between W, H and input parameters.

For the simplicity, $P_{O_1 B} = l_1$ and $P_{O_2 C} = l_2$ are defined.
$l_1$ is not the input parameter,
but it can be calculated from $P_{O_1 A}$ and $\theta_1$ and $\theta_2$ as described above.

The projection $O_1 O_2$ to $\boldsymbol{u}_3 = (-\sin (\alpha/2), -\cos (\alpha/2))$
is $(W, -H)\cdot(\sin\alpha/2, -\cos\alpha/2) = W\sin\alpha/2+H\cos\alpha/2$

The projection of BC to $u_3$ is $P_{BC} \cos(\pi/2-\theta_3) =P_{BC}\sin\theta_3$.
As 
$$
W\sin(\alpha/2) + H \cos(\alpha/2) = P_{BC} \sin \theta_3 + l_1 + l_2
$$

$$
\begin{aligned}
l_1 + l_2 &= W\sin(\alpha/2) + H \cos(\alpha/2) - P_{BC} \sin \theta_3 \\
&= W\sin(\alpha/2) + H \cos(\alpha/2) - \frac{W \cos (\alpha/2) - H \sin (\alpha/2)}{\cos \theta_3} \sin \theta_3 \\
&= \frac{W\sin( \alpha/2 )\cos\theta_3+H\cos( \alpha/2 )\cos\theta_3-W\cos( \alpha/2 )\sin\theta_3+H\sin( \alpha/2 )\sin\theta_3}{\cos\theta_3} \\
&= \frac{1}{\cos\theta_3} \left( W(\sin(\alpha/2 - \theta_3)+ H(\cos(\theta_3 - \alpha/2 ) \right) \\
&= \frac{H \cos(\theta_3 - \alpha/2) - W \sin(\theta_3 -\alpha/2 )}{\cos \theta_3}
\end{aligned}
$$

```{python}

import sympy as sp
from sympy import symbols, solve, factor, simplify, tan, cos, sin,  sec, trigsimp, expand_trig
sp.init_printing()

alpha, theta3, l1, l2, W, H, t, t2, s, pbc = symbols('alpha theta3 l1 l2 W H t t2 s pbc', real=True, positive=True)

eq_slop: sp.Expr = tan(alpha/2 - theta3) - ((-H + l2*cos(alpha/2) + l1*cos(alpha/2)) / 
                               (W - l2*sin(alpha/2) - l1*sin(alpha/2)))
eq1: sp.Expr = H* cos(theta3-alpha/2)- W*sin(theta3 -alpha/2) - (l1 + l2)*cos(theta3)
eq2: sp.Expr = t - (W*sin(alpha/2) + H*cos(alpha/2))
eq3: sp.Expr = t2 - (W*cos(alpha/2) + H*sin(alpha/2))
eq4: sp.Expr = s  - (W*sin(alpha/2) - H*cos(alpha/2))
eq5: sp.Expr = pbc * cos(theta3)- (W*cos(alpha/2) - H*sin(alpha/2))

sols_t: sp.Expr = solve([eq1, eq2], [W, H])
sols_t2: sp.Expr = solve([eq1, eq3], [W, H])
sols_s: sp.Expr = solve([eq1, eq4], [W, H])
sols_pbc = sp.Expr = solve([eq1, eq5], [W, H])

clean_sols_t = {var: trigsimp(expand_trig(expr)) for var, expr in sols_t.items()}
clean_sols_t2 = {var: trigsimp(expand_trig(expr)) for var, expr in sols_t2.items()}
clean_sols_s =  {var: trigsimp(expand_trig(expr)) for var, expr in sols_s.items()}
clean_sols_pbc =  {var: trigsimp(expand_trig(expr)) for var, expr in sols_pbc.items()}

clean_sols_pbc
```


```{python}
clean_sols_t[W]
```
```{python}
clean_sols_t[H]
```

# Derivatives of optical path with respect to wavelength

## Path in prism (AB and CD) 

From @eq-PAB, $\frac{d^2P_{AB}}{d\lambda^2}$ is calculated as follows:
Note that $\frac{n}{\cos \theta_2}$ depends on $\lambda$ through $\theta_2$ and $n$.
The second derivative of $\frac{n(\lambda)}{\cos \theta (\lambda)}$ by $\lambda$ is :
```{python}
#| echo: false
lamb = sp.symbols('lambda', real=True, positive=True)
n = sp.Function('n', real=True)(lamb)
theta = sp.Function('theta', real=True)(lamb)

expr = n/sp.cos(theta)

d_expr = sp.diff(expr, lamb, 2)

trigsimp(expand_trig(d_expr))
```

$\theta_2 = \alpha - \sin^{-1}(\frac{\sin \theta_0}{n})$
(Because of Snell's law: $\frac{\sin \theta_1}{n} = \sin \theta_1 = \sin(\alpha - \theta_2)$)

From @eq-PCD, we consider the derivative of $\frac{n(\lambda)}{\cos \theta_1(\lambda)}$ similarly.
$\theta_1 = \sin^{-1}(\frac{\sin \theta_0}{n})$

Thus, the (positive) GDD arising from the propagation through the prism and (negative) contribution because of 
the angular dispersion ($d\theta_1/d\lambda$) over the medium can be calculated.

## Path in air (BC)
From @eq-PBC, $\frac{d^2 P_{BC}}{d \lambda^2}$ is calculated as follows:
the numerator does not depend on $\lambda$, thus only the derivative of $\frac{1}{\cos \theta_3}$ is calculated here.
The second derivative of it is as follows:
```{python}
#| echo: false
expr_2 = 1/sp.cos(theta)
d_expr_2 = sp.diff(expr_2, lamb, 2)
trigsimp(expand_trig(d_expr_2))
```

and 
$\theta_3 = \sin^{-1}(n \sin(\alpha - \sin^{-1}(\frac{\sin \theta_0}{n}) ))$,
thus, the (negative) GDD arising from the angular dispersion in the air gap can be calculated.
( All refraction angles are defined positive when measured counterclockwise from the surface normal.)

The rest is basically a coding issue.

# The special case: Brewster angle prism pair
Before going to forward calculations, let us consider the special case of the prism pair where the apex angle
is $\alpha = \pi - 2 \theta_B = \pi-2 \tan^{-1}n$, where $\theta_B$ is the Brewster angle.
And suppose that the incident angle $\theta_0$ is the Brewster angle, i.e., $\theta_0=\theta_B=\tan^{-1}( n)$.
In this case, $\theta_0 = \theta_3 = \theta_4 = \theta_7 = \theta_B$, and $\theta_1 = \theta_2 = \theta_5 = \theta_6 = \alpha/2  = \pi/2 - \theta_B$


